theories/Index/Index.v
@@ -30,6 +30,7 @@ Require Import PnV.Logic.PropositionalLogic.
 Require Import PnV.System.BasicITreeTh.
 Require Import PnV.System.FolFramework.
 Require Import PnV.System.Lambda1.
+Require Import PnV.System.Lang.
 Require Import PnV.System.P.
 Require Import PnV.System.Regex.
 Require Import PnV.System.STLC.
