theories/System/Lang.v
@@ -1,0 +1,196 @@
+Require Import PnV.Prelude.Prelude.
+Require Import PnV.Math.ThN.
+Require Import PnV.System.P.
+
+Module LANG1.
+
+Variant alphabet : Set :=
+  | L
+  | R.
+
+#[local] Notation string := (list alphabet).
+#[local] Notation lang := (ensemble string).
+#[local] Infix " \in " := E.In : type_scope.
+
+#[local]
+Instance alphabet_hasEqDec
+  : hasEqDec alphabet.
+Proof.
+  red. decide equality.
+Defined.
+
+Inductive L_cfg1 : lang :=
+  | cfg1_rule1
+    : [] \in L_cfg1
+  | cfg1_rule2 (str: string)
+    (H_str: str \in L_cfg1)
+    : [L] ++ str ++ [R] \in L_cfg1
+  | cfg1_rule3 (str: string)
+    (H_str: str \in L_cfg1)
+    : [R] ++ str ++ [L] \in L_cfg1
+  | cfg1_rule4 (str1: string) (str2: string)
+    (H_str1: str1 \in L_cfg1)
+    (H_str2: str2 \in L_cfg1)
+    : str1 ++ str2 \in L_cfg1.
+
+#[local] Hint Constructors L_cfg1 : core.
+
+Notation count a s := (count_occ eq_dec s a).
+
+Variant cfg1_spec (LANG: lang) : Prop :=
+  | cfg1_lang_spec
+    (nL_eq_nR: forall str, str \in LANG <-> count L str = count R str)
+    : cfg1_spec LANG.
+
+Section THEORY.
+
+Lemma count_app a s s'
+  : count a (s ++ s') = count a s + count a s'.
+Proof.
+  revert a s'; induction s as [ | [ | ] s IH]; intros [ | ] s'; simpl; eauto.
+Qed.
+
+Lemma count_app_cancel_l a s s' n n'
+  (H_s_app_s' : count a (s ++ s') = n + n')
+  (H_s : count a s = n)
+  : count a s' = n'.
+Proof.
+  revert a s' n n' H_s_app_s' H_s; induction s as [ | [ | ] s IH]; intros [ | ]; simpl; i; subst n; eauto.
+Qed.
+
+Lemma count_app_cancel_r a s s' n n'
+  (H_s_app_s' : count a (s ++ s') = n + n')
+  (H_s' : count a s' = n')
+  : count a s = n.
+Proof.
+  subst n'. revert a s' n H_s_app_s'. induction s' as [ | [ | ] s' IH] using List.rev_ind; simpl; i.
+  all: try rewrite Nat.add_0_r in *; try rewrite app_nil_r in *; eauto.
+  all: erewrite count_occ_app with (l1 := s) (l2 := s' ++ [_]) in H_s_app_s'; lia.
+Qed.
+
+Lemma cfg1_soundness s
+  (H_in : s \in L_cfg1)
+  : count L s = count R s.
+Proof with eauto.
+  induction H_in as [ | s1 H_in1 IH1 | s2 H_in2 IH2 | s1 s2 H_in1 IH1 H_in2 IH2]; simpl...
+  - rewrite <- rev_involutive with (l := _ ++ [_]). rewrite rev_unit.
+    do 2 rewrite count_occ_rev. simpl. do 2 rewrite count_occ_rev...
+  - rewrite <- rev_involutive with (l := _ ++ [_]). rewrite rev_unit.
+    do 2 rewrite count_occ_rev. simpl. do 2 rewrite count_occ_rev...
+  - do 2 rewrite count_occ_app...
+Qed.
+
+Inductive isLast a : string -> Prop :=
+  | isLast_1
+    : isLast a [a]
+  | isLast_S (a': alphabet) (s: string)
+    (H_isLast: isLast a s)
+    : isLast a (a' :: s).
+
+#[local] Hint Constructors isLast : core.
+
+Lemma isLast_elim a s
+  (H_isLast : isLast a s)
+  : exists s', s = s' ++ [a].
+Proof.
+  induction H_isLast as [ | a' s H_isLast [s' IH]].
+  - exists []; eauto.
+  - rewrite IH. exists (a' :: s'). reflexivity.
+Qed.
+
+Variant string_cut s : Prop :=
+  | string_cut_intro s_prefix s'
+    (H_app : s = s_prefix ++ s')
+    (H_len : length s' > 0)
+    (H_cut : count L s' = count R s')
+    : string_cut s.
+
+Lemma if_count_L_s_lt_count_R_s s
+  (count_L_s_lt_count_R_s : count L s < count R s)
+  : string_cut s \/ isLast R s.
+Proof with eauto.
+  revert count_L_s_lt_count_R_s; set (black := L); set (white := R).
+  induction s as [ | [ | ] s IHs]; simpl; try lia; i.
+  - assert (IH : count black s < count white s) by lia.
+    apply IHs in IH. destruct IH as [IH | IH]...
+    inversion IH; subst. left. eapply string_cut_intro with (s' := s') (s_prefix := black :: s_prefix)...
+  - assert (count black s = count white s \/ count black s < count white s) as [IH | IH] by lia.
+    + destruct s as [ | a' s']...
+      left. eapply string_cut_intro with (s' := a' :: s') (s_prefix := [white])... simpl; lia.
+    + apply IHs in IH. destruct IH as [IH | IH]...
+      left. inversion IH; subst. eapply string_cut_intro with (s' := s') (s_prefix := white :: s_prefix)...
+Qed.
+
+Lemma if_count_L_s_gt_count_R_s s
+  (count_L_s_gt_count_R_s : count L s > count R s)
+  : string_cut s \/ isLast L s.
+Proof with eauto.
+  revert count_L_s_gt_count_R_s; set (black := R); set (white := L).
+  induction s as [ | [ | ] s IHs]; simpl; try lia; i; cycle -1.
+  - assert (IH : count black s < count white s) by lia.
+    apply IHs in IH. destruct IH as [IH | IH]...
+    inversion IH; subst. left. eapply string_cut_intro with (s' := s') (s_prefix := black :: s_prefix)...
+  - assert (count black s = count white s \/ count black s < count white s) as [IH | IH] by lia.
+    + destruct s as [ | a' s']...
+      left. eapply string_cut_intro with (s' := a' :: s') (s_prefix := [white])... simpl; lia.
+    + apply IHs in IH. destruct IH as [IH | IH]...
+      left. inversion IH; subst. eapply string_cut_intro with (s' := s') (s_prefix := white :: s_prefix)...
+Qed.
+
+Theorem cfg1_completeness s
+  (count_L_eq_count_R : count L s = count R s)
+  : s \in L_cfg1.
+Proof with eauto.
+  revert count_L_eq_count_R. pose proof (relation_on_image_liftsWellFounded lt (@length alphabet) lt_wf s) as H_ACC.
+  unfold binary_relation_on_image in H_ACC. induction H_ACC as [[ | [ | ] s] _ IHs]; simpl in *; i...
+  - assert (count_L_s_lt_count_R_s : count L s < count R s) by lia.
+    apply if_count_L_s_lt_count_R_s in count_L_s_lt_count_R_s.
+    destruct count_L_s_lt_count_R_s as [[? ? ? ? ?] | H_last_R].
+    + assert (IH1 : length s' < S (length s)) by now pose proof (@length_app _ s_prefix s'); subst s; lia.
+      pose proof (IHs s' IH1 H_cut) as H_s'.
+      assert (IH2: length (L :: s_prefix) < S (length s)) by now simpl; pose proof (@length_app _ s_prefix s'); subst s; lia.
+      assert (CLAIM : count L (L :: s_prefix) = count R (L :: s_prefix)).
+      { eapply count_app_cancel_r with (s := L :: s_prefix) (s' := s') (n' := count R s')...
+        simpl. rewrite <- H_app. rewrite <- count_app. rewrite <- H_app...
+      }
+      assert (H_prefix : L :: s_prefix \in L_cfg1)...
+      rewrite H_app. eapply cfg1_rule4 with (str1 := L :: s_prefix) (str2 := s')...
+    + apply isLast_elim in H_last_R. destruct H_last_R as [s' ->]; simpl in *. eapply cfg1_rule2. eapply IHs.
+      * replace (length (s' ++ [R])) with (length (rev (R :: rev s'))) by now simpl; f_equal; rewrite rev_involutive.
+        rewrite length_rev. simpl. rewrite length_rev. lia.
+      * rewrite <- rev_involutive with (l := s' ++ [R]) in count_L_eq_count_R.
+        rewrite -> rev_unit in count_L_eq_count_R. do 2 rewrite count_occ_rev in count_L_eq_count_R.
+        simpl in count_L_eq_count_R. apply f_equal with (f := Nat.pred) in count_L_eq_count_R.
+        simpl in count_L_eq_count_R. do 2 rewrite count_occ_rev in count_L_eq_count_R...
+  - assert (count_L_s_gt_count_R_s : count L s > count R s) by lia.
+    apply if_count_L_s_gt_count_R_s in count_L_s_gt_count_R_s.
+    destruct count_L_s_gt_count_R_s as [[? ? ? ? ?] | H_last_L].
+    + assert (IH1 : length s' < S (length s)) by now pose proof (@length_app _ s_prefix s'); subst s; lia.
+      pose proof (IHs s' IH1 H_cut) as H_s'.
+      assert (IH2 : length (R :: s_prefix) < S (length s)) by now simpl; pose proof (@length_app _ s_prefix s'); subst s; lia.
+      assert (CLAIM : count L (R :: s_prefix) = count R (R :: s_prefix)).
+      { eapply count_app_cancel_r with (s := R :: s_prefix) (s' := s') (n' := count R s')...
+        simpl. rewrite <- H_app. rewrite <- count_app. rewrite <- H_app...
+      }
+      assert (H_prefix : R :: s_prefix \in L_cfg1)...
+      rewrite H_app. eapply cfg1_rule4 with (str1 := R :: s_prefix) (str2 := s')...
+    + apply isLast_elim in H_last_L. destruct H_last_L as [s' ->]; simpl in *. eapply cfg1_rule3. eapply IHs.
+      * replace (length (s' ++ [L])) with (length (rev (L :: rev s'))) by now simpl; f_equal; rewrite rev_involutive.
+        rewrite length_rev. simpl. rewrite length_rev. lia.
+      * rewrite <- rev_involutive with (l := s' ++ [L]) in count_L_eq_count_R.
+        rewrite -> rev_unit in count_L_eq_count_R. do 2 rewrite count_occ_rev in count_L_eq_count_R.
+        simpl in count_L_eq_count_R. apply f_equal with (f := Nat.pred) in count_L_eq_count_R.
+        simpl in count_L_eq_count_R. do 2 rewrite count_occ_rev in count_L_eq_count_R...
+Qed.
+
+Corollary L_cfg1_satisfies_its_spec
+  : cfg1_spec L_cfg1.
+Proof.
+  constructor. intros s. split.
+  - exact (cfg1_soundness s).
+  - exact (cfg1_completeness s).
+Qed.
+
+End THEORY.
+
+End LANG1.
